feat: improve json parsing, introduce unicode_str and unicode codepoint handling

src/json.v
@@ -1,41 +1,75 @@
-From Coq Require Import Strings.String.
 From Coq Require Import Strings.Ascii.
+From Coq Require Import Strings.Byte.
 From Coq Require Import ZArith.
 
 From Coq Require Import Lists.List. Import ListNotations.
 
 Open Scope char_scope.
 
+Inductive nonzero :=
+| D1 | D2 | D3
+| D4 | D5 | D6
+| D7 | D8 | D9.
+
+Inductive digit :=
+| Zero
+| NonZero : nonzero -> digit.
+
+Inductive sign :=
+| Positive
+| Negative.
+
+Inductive integer :=
+| IntegerZero
+| MoreThanZero (first_digit: nonzero) (rest_digits: list digit).
+
+Record exponent := {
+    exponent_sign: option sign;
+    first_digit: digit;
+    digits: list digit
+  }.
+
+Record number := {
+    negative: bool;
+    integer_part: integer;
+    fractional_part: list digit;
+    exponent_part: option exponent
+  }.
+
+Definition codepoint : Type := (byte * byte * byte * byte).
+Definition unicode_str : Type := list codepoint.
+
 Inductive json : Type :=
 | JNull
 | JTrue
 | JFalse
-| JNumber : nat -> json
-| JString : string -> json
-| JList   : list json -> json
-| JObject : list (string * json) -> json.
+| JNumber (n: number)
+| JString (s: unicode_str)
+| JList   (l: list json)
+| JObject (obj: list (unicode_str * json)).
 
-Inductive ParserError :=
+Definition codepoint_eqb (a b: codepoint) : bool :=
+  let '(a1, a2, a3, a4) := a in
+  let '(b1, b2, b3, b4) := b in
+  (eqb a1 b1) && (eqb a2 b2) && (eqb a3 b3) && (eqb a4 b4).
+
+Definition from_ascii (c: ascii) : codepoint :=
+  let b := byte_of_ascii c in
+  (b, x00, x00, x00).
+
+Inductive error_message :=
 | UnexpectedEOF
-| Expected (c: ascii) (got: ascii).
+| UnexpectedChar (c: codepoint)
+| ExpectedChar (c: codepoint) (got: codepoint).
 
-Inductive Result {T} : Type :=
-| Ok (x: T) : @Result T
-| Err (err: ParserError) : @Result T.
+Inductive result {T E: Type} : Type :=
+| Ok (x: T) : @result T E
+| Err (err: E) : @result T E.
 
-Arguments Ok {T}.
-Arguments Err {T}.
+Arguments Ok {T E}.
+Arguments Err {T E}.
 
-Definition parser {T} := string -> @Result (T * string).
-
-Definition map {A B} (f: A -> B) (p: @parser A) : @parser B :=
-  fun s =>
-    match p s with
-    | Ok (x, rest) => Ok (f x, rest)
-    | Err err => Err err
-    end.
-
-Definition bind {A B} (r: @Result A) (f: A -> @Result B) :=
+Definition bind {A B E} (r: @result A E) (f: A -> @result B E) :=
   match r with
   | Ok p => f p
   | Err err => Err err
@@ -45,103 +79,170 @@ Notation "'let*' p ':=' c1 'in' c2" :=
   (bind c1 (fun p => c2))
     (at level 61, p as pattern, c1 at next level, right associativity).
 
-Lemma n_not_less_than_10 : forall n, 10 + n < 10 -> False.
-Proof.
-  intros.
-  repeat apply PeanoNat.lt_S_n in H.
-  apply Nat.nlt_0_r in H. apply H.
-Defined.
+Definition fmap { A B E } (f: A -> B) (r: @result A E) : @result B E :=
+  bind r (fun x => Ok (f x)).
 
-Definition ascii_of_nat (s: {n: nat | n < 10}) : ascii :=
-  match s with
-  | exist _ 0 _ => "0"
-  | exist _ 1 _ => "1"
-  | exist _ 2 _ => "2"
-  | exist _ 3 _ => "3"
-  | exist _ 4 _ => "4"
-  | exist _ 5 _ => "5"
-  | exist _ 6 _ => "6"
-  | exist _ 7 _ => "7"
-  | exist _ 8 _ => "8"
-  | exist _ 9 _ => "9"
-  | exist _ _ p => match n_not_less_than_10 _ p with end
-  end.
+Definition parser {T: Type} := unicode_str -> @result (T * unicode_str) (list error_message).
 
-Definition mod_10 (n: nat) : { m: nat | m < 10}.
-Proof.
-  intros.
-  refine (exist _ (n mod 10) _).
-  apply Nat.mod_upper_bound. apply Nat.neq_succ_0.
-Defined.
+Definition parser_map {A B} (f: A -> B) (p: @parser A) : @parser B :=
+  fun s =>
+    let* (x, rest) := p s in
+    Ok (f x, rest).
 
-Fixpoint string_of_nat_aux (time n : nat) (acc : string) : string :=
-  let d := ascii_of_nat (mod_10 n) in
-  let acc' := String d acc in
-  match time with
-    | 0 => acc'
-    | S time' =>
-      match n / 10 with
-        | 0 => acc'
-        | n' => string_of_nat_aux time' n' acc'
-      end
-  end.
+Definition maybe {A} (p: @parser A) : @parser (option A) :=
+  fun s =>
+    match p s with
+    | Ok (x, rest) => Ok (Some x, rest)
+    | Err _        => Ok (None, s)
+    end.
 
-Definition string_of_nat (n : nat) : string :=
-  string_of_nat_aux n n EmptyString.
+Fixpoint any_aux {A} (parsers: list (@parser A)) (errs: list error_message) : @parser A :=
+  fun s =>
+    match parsers with
+    | [] => Err errs
+    | p :: rest =>
+        match p s with
+        | Err err => any_aux rest (err ++ errs) s
+        | Ok p => Ok p
+        end
+    end.
 
-Definition nat_of_ascii (char: ascii) : option nat :=
-  match char with
-  | "0" => Some 0
-  | "1" => Some 1
-  | "2" => Some 2
-  | "3" => Some 3
-  | "4" => Some 4
-  | "5" => Some 5
-  | "6" => Some 6
-  | "7" => Some 7
-  | "8" => Some 8
-  | "9" => Some 9
-  | _ => None
-  end.
+Definition any {A} (parsers : list (@parser A)): @parser A := any_aux parsers [].
 
-Fixpoint nat_of_string_aux (acc: nat) (s: string) : @Result (nat * string) :=
-  match s with
-  | EmptyString => Ok (acc, s)
-  | String c s' =>
-      match nat_of_ascii c with
-      | Some n => nat_of_string_aux (10 * acc + n) s'
-      | None => Err UnexpectedEOF
-      end
-  end.
+Definition predicate (pred: codepoint -> bool) (err: codepoint -> error_message) : @parser codepoint :=
+  fun s => 
+    match s with
+    | [] => Err [ UnexpectedEOF ]
+    | c :: rest =>
+        match pred c with
+        | true => Ok (c, rest)
+        | false => Err [ err c ]
+        end
+    end.
 
-Definition parse_nat : @parser nat :=
-  fun s => nat_of_string_aux 0 s.
+Definition expect (c: ascii) : @parser codepoint :=
+  predicate (codepoint_eqb (from_ascii c)) UnexpectedChar.
 
-Open Scope string_scope.
-Definition serialize_json (obj: json) : option string :=
+Definition not (c: ascii) : @parser codepoint :=
+  predicate (fun c' => negb (codepoint_eqb (from_ascii c) c')) (ExpectedChar (from_ascii c)).
+
+Fixpoint many_aux { A } (p: @parser A) (acc: list A) (fuel: nat) : @parser (list A) :=
+  fun s => 
+    match fuel with
+    | 0 => Ok (acc, s)
+    | S fuel' =>
+        match p s as res with
+        | Ok (val, rest) => many_aux p (val :: acc) fuel' rest
+        | Err _ => Ok (acc, s)
+        end
+    end.
+
+Definition many {A} (p: @parser A): @parser (list A) :=
+  fun s => many_aux p [] (S (length s)) s.
+
+(* ============================================== *)
+(* JSON parser implementation                     *)
+(* ============================================== *)
+
+Definition parse_nonzero : @parser nonzero :=
+  let p digit char := parser_map (fun _ => digit) (expect char) in
+  any [
+      p D1 "1"; p D2 "2"; p D3 "3";
+      p D4 "4"; p D5 "5"; p D6 "6";
+      p D7 "7"; p D8 "8"; p D9 "9"
+    ].
+
+Definition parse_digit : @parser digit :=
+  let z := parser_map (fun _ => Zero) (expect "0") in
+  let n := parser_map NonZero parse_nonzero in
+  any [z; n].
+
+Definition parse_integer : @parser integer :=
+  let parse_integer_zero := parser_map (fun _ => IntegerZero) (expect "0") in
+  let parse_more_than_zero :=
+    fun s =>
+      let* (fst, rest) := parse_nonzero s in
+      let* (rest_digits, rest) := many parse_digit rest in
+      Ok (MoreThanZero fst rest_digits, rest) in
+  any [ parse_integer_zero; parse_more_than_zero ].
+
+Definition parse_fraction: @parser (list digit) :=
+  fun s =>
+    let* (_dot, rest) := expect "." s in
+    let* (digits, rest) := many parse_digit rest in
+    Ok (digits, rest).
+
+Definition parse_sign : @parser sign :=
+  any [ parser_map (fun _ => Negative) (expect "-");
+        parser_map (fun _ => Positive) (expect "+") ].
+
+Definition parse_exponent: @parser exponent :=
+  fun s =>
+    let* (_e, rest) := any [ expect "e"; expect "E" ] s in
+    let* (sign, rest) := maybe parse_sign rest in
+    let* (fst_digit, rest) := parse_digit rest in
+    let* (digits, rest) := many parse_digit rest in
+    Ok( {| exponent_sign := sign; digits:= digits; first_digit:= fst_digit |}, rest).
+
+Definition parse_number: @parser number :=
+  fun s =>
+    let* (negative, rest) := maybe (expect "-") s      in
+    let* (integer, rest)  := parse_integer rest        in
+    let* (fraction, rest) := maybe parse_fraction rest in
+    let* (exponent, rest) := maybe parse_exponent rest in
+    Ok({|
+          negative := match negative with Some _ => true| None => false end;
+          integer_part := integer;
+          fractional_part := match fraction with Some l => l | None => [] end;
+          exponent_part := exponent
+        |}, rest).
+
+Require Extraction.
+Extraction parse_number.
+
+Definition serialize_json (obj: json) : unicode_str :=
   match obj with
-  | JNull => Some "null"
-  | JTrue => Some "true"
-  | JFalse => Some "false"
-  | JNumber n => Some (string_of_nat n)
-  | _ => None
+  | JNull => "null"
+  | JTrue => "true"
+  | JFalse => "false"
+  | JNumber n => string_of_nat n
+  | JString s => String "034"%char (s ++ (String "034"%char EmptyString))
+  | _ => ""
   end.
+
+Compute (serialize_json (JString "hello world")).
 Close Scope string_scope.
 
-Definition parse_null: @parser json :=
+Definition parse_constant (c: json) : @parser json :=
+  let const_string := serialize_json c in 
   fun s =>
-    if prefix "null" s then
-      Ok((JNull, substring 4 (String.length s) s))
-    else Err UnexpectedEOF.
+    if prefix const_string s then
+      Ok((c, substring (String.length const_string) (String.length s) s))
+    else
+      Err (Message "Expected " ++ const_string).
+                        
+Definition parse_null: @parser json := parse_constant JNull.
+Definition parse_true: @parser json := parse_constant JTrue.
+Definition parse_false: @parser json := parse_constant JFalse.
 
-Definition parse_true: @parser json :=
+Definition parse_string: @parser json :=
   fun s =>
-    if prefix "true" s then
-      Ok((JTrue, substring 4 (String.length s) s))
-    else Err UnexpectedEOF.
+    let* (_, rest) := expect """" s in
+    let* (s, rest) := many (not """") rest in
+    let* (_, rest) := expect """" rest in
+    Ok (JString (string_of_list_ascii (rev s)), rest).
 
-Definition parse_false: @parser json :=
-  fun s =>
-    if prefix "false" s then
-      Ok((JFalse, substring 5 (String.length s) s))
-    else Err UnexpectedEOF.
+Definition parse_object_aux (fuel: nat) (acc: list (string * json)) : @parser json := 
+
+Definition parse_object: @parser json := 
+
+Compute (parse_string (serialize_json (JString "hello world"))).
+
+Definition parse_value : @parser json :=
+  any [
+      parse_number;
+      parse_string;
+      parse_null;
+      parse_true;
+      parse_false
+    ].
