src/json_theorems.v
@@ -53,12 +53,35 @@ Open Scope string_scope.
 Theorem parse_null_isomorphic : parse_null "null" = Ok((JNull, "")).
   reflexivity.
 Qed.
-
 Theorem parse_true_isomorphic : parse_true "true" = Ok((JTrue, "")).
   reflexivity.
 Qed.
-
 Theorem parse_false_isomorphic : parse_false "false" = Ok((JFalse, "")).
   reflexivity.
 Qed.
 
+Theorem parser_map_correct { A B }: forall (f: A -> B) (p: @parser A) (s: string),
+    parser_map f p s = fmap (fun '(x, rest) => (f x, rest)) (p s).
+Proof.
+  intros.
+  unfold parser_map.
+  cbv delta. f_equal; simpl.
+  destruct (p s); try destruct x; reflexivity.
+Qed.
+
+Theorem parse_number_isomorphic :forall n, parse_number (serialize_json (JNumber n)) = Ok((JNumber n, "")).
+Proof.
+  intros.
+  unfold parse_number, serialize_json.
+  rewrite parser_map_correct.
+  rewrite parse_nat_isomorphic.
+  reflexivity.
+Defined.
+
+Theorem parse_correct_left (j: json) : parse_json (serialize_json j) = Ok((j, "")).
+Proof.
+  induction j; try auto.
+  - unfold parse_json. unfold one_of. rewrite parse_number_isomorphic. reflexivity.
+  - 
+  
+  
